RegexCorrectness/NFA/Transition/Closure/Equivalence.lean
@@ -6,18 +6,6 @@ import Mathlib.Data.List.Indexes
 
 namespace Regex.NFA
 
-theorem εClosure_of_pathIn {nfa : NFA} {start} (path : nfa.pathIn start i i' []) :
-  i' ∈ nfa.εClosure i := by
-  generalize h : [] = cs at path
-  induction path with
-  | base _ => exact .base
-  | @step i j k cs cs' step _ ih =>
-    simp at h
-    simp [h] at *
-    cases step with
-    | εStep _ _ step =>
-      exact εClosure.step (εStep_of_εStep step) ih
-
 theorem εClosure_of_pathIn' {nfa : NFA} (path : nfa.pathIn' lb i i' []) :
   i' ∈ nfa.εClosure i := by
   generalize h : [] = cs at path
@@ -32,20 +20,6 @@ theorem εClosure_of_pathIn' {nfa : NFA} (path : nfa.pathIn' lb i i' []) :
     cases step with
     | εStep _ _ step =>
       exact εClosure.step (εStep_of_εStep step) ih
-
-theorem pathIn_iff_εClosure {nfa : NFA} :
-  nfa.pathIn 0 i i' [] ↔ i' ∈ nfa.εClosure i := by
-  apply Iff.intro
-  . exact εClosure_of_pathIn
-  . intro h
-    induction h with
-    | base => exact .base (Nat.zero_le _)
-    | @step i j k step _ ih =>
-      cases Nat.decLt i nfa.nodes.size with
-      | isTrue lt =>
-        simp [εStep, lt] at step
-        exact .step (.εStep (Nat.zero_le _) lt step) ih
-      | isFalse nlt => simp [εStep, nlt] at step
 
 theorem eq_or_pathIn'_of_εClosure {nfa : NFA} (cls : i' ∈ nfa.εClosure i) :
   i = i' ∨ nfa.pathIn' 0 i i' [] := by
@@ -62,40 +36,6 @@ theorem eq_or_pathIn'_of_εClosure {nfa : NFA} (cls : i' ∈ nfa.εClosure i) :
         | inr path =>
           exact .inr (.more (.εStep (Nat.zero_le _) lt step) path)
       | isFalse nlt => simp [εStep, nlt] at step
-
-theorem pathIn.of_snoc_char {start}
-  (path : pathIn nfa start i l (cs ++ [c])) :
-  ∃ j k, pathIn nfa start i j cs ∧ k ∈ nfa.charStep j c ∧ l ∈ nfa.εClosure k := by
-  generalize h : cs ++ [c] = cs' at path
-  induction path generalizing cs with
-  | base _ => simp at h
-  | @step i j k cs₁ cs₂ step rest ih =>
-    match snoc_eq_append h with
-    | .inl ⟨h₁, h₂⟩ =>
-      simp [h₁, h₂] at step rest
-      have := step.nil_of_snoc
-      simp [this] at *
-      cases step with
-      | charStep le _ step =>
-        exact ⟨i, .base le, j, charStep_of_charStep step, εClosure_of_pathIn rest⟩
-    | .inr ⟨cs₂', h₁, h₂⟩ =>
-      have ⟨j', k', path', step', cls⟩ := ih h₂.symm
-      exact ⟨j', k', h₁ ▸ .step step path', step', cls⟩
-where
-  snoc_eq_append {cs₁ cs₂ cs₃ : List Char} {c : Char} (h : cs₁ ++ [c] = cs₂ ++ cs₃) :
-    (cs₂ = cs₁ ++ [c] ∧ cs₃ = []) ∨ (∃ cs₃', cs₁ = cs₂ ++ cs₃' ∧ cs₃ = cs₃' ++ [c]) := by
-    cases cs₃ using List.list_reverse_induction with
-    | base =>
-      simp at h
-      exact .inl ⟨h.symm, rfl⟩
-    | ind cs₃ c' =>
-      have : c = c' ∧ cs₁ = cs₂ ++ cs₃ := by
-        have h₁ := congrArg List.reverse h
-        simp at h₁
-        have h₂ := congrArg List.reverse h₁.right
-        simp at h₂
-        exact ⟨h₁.left, h₂⟩
-      simp [this]
 
 -- TODO: explain
 theorem pathIn'.of_snoc_char (assm : cs' = cs ++ [c])
@@ -114,7 +54,7 @@ theorem pathIn'.of_snoc_char (assm : cs' = cs ++ [c])
       exact ⟨0, j, .inl (.charStep h₁ h₂ step), .inl rfl⟩
     | εStep => simp at assm
   | @more i j k cs₁ cs₂ step rest ih =>
-    match pathIn.of_snoc_char.snoc_eq_append assm.symm with
+    match snoc_eq_append assm.symm with
     | .inl ⟨h₁, h₂⟩ =>
       simp [h₁, h₂] at step rest
       have := step.nil_of_snoc
@@ -131,20 +71,21 @@ theorem pathIn'.of_snoc_char (assm : cs' = cs ++ [c])
       | .inr ⟨path', step'⟩ =>
         simp [h₁]
         exact ⟨j', k', .inr ⟨.more step path', step'⟩, h₄⟩
-
-theorem pathIn_of_reaches {nfa : NFA} {i : Fin nfa.nodes.size} {m : List Char}
-  (h : nfa.reaches i m) :
-  nfa.pathIn 0 nfa.start i m := by
-  induction h with
-  | nil cls => simp [pathIn_iff_εClosure.mpr cls]
-  | @snoc i j k c m _ step cls ih =>
-    simp [charStep] at step
-    have ih' : nfa.pathIn (min 0 j) nfa.start j (m ++ [c]) :=
-      ih.snoc_char i.isLt step
-    simp at ih'
-    have := ih'.trans (pathIn_iff_εClosure.mpr cls)
-    simp at this
-    exact this
+where
+  snoc_eq_append {cs₁ cs₂ cs₃ : List Char} {c : Char} (h : cs₁ ++ [c] = cs₂ ++ cs₃) :
+    (cs₂ = cs₁ ++ [c] ∧ cs₃ = []) ∨ (∃ cs₃', cs₁ = cs₂ ++ cs₃' ∧ cs₃ = cs₃' ++ [c]) := by
+    cases cs₃ using List.list_reverse_induction with
+    | base =>
+      simp at h
+      exact .inl ⟨h.symm, rfl⟩
+    | ind cs₃ c' =>
+      have : c = c' ∧ cs₁ = cs₂ ++ cs₃ := by
+        have h₁ := congrArg List.reverse h
+        simp at h₁
+        have h₂ := congrArg List.reverse h₁.right
+        simp at h₂
+        exact ⟨h₁.left, h₂⟩
+      simp [this]
 
 theorem eq_or_pathIn'_of_reaches {nfa : NFA} {i : Fin nfa.nodes.size} {m : List Char}
   (h : nfa.reaches i m) :
@@ -174,17 +115,6 @@ theorem eq_or_pathIn'_of_reaches {nfa : NFA} {i : Fin nfa.nodes.size} {m : List 
         simp at this
         exact .inr this
 
-theorem reaches_of_pathIn {nfa : NFA} {i : Fin nfa.nodes.size} {m : List Char}
-  (h : nfa.pathIn 0 nfa.start i m) :
-  nfa.reaches i m := by
-  induction m using List.list_reverse_induction generalizing i with
-  | base => exact .nil (pathIn_iff_εClosure.mp h)
-  | ind m c ih =>
-    have ⟨j, k, path, step, cls⟩ := pathIn.of_snoc_char h
-    let j' : Fin nfa.nodes.size := ⟨j, path.lt_right nfa.start.isLt⟩
-    have prev := ih (i := j') path
-    exact .snoc prev step cls
-
 theorem reaches_of_pathIn' {nfa : NFA} {i : Fin nfa.nodes.size} {m : List Char}
   (h : nfa.pathIn' 0 nfa.start i m) :
   nfa.reaches i m := by
@@ -207,18 +137,6 @@ theorem reaches_of_pathIn' {nfa : NFA} {i : Fin nfa.nodes.size} {m : List Char}
       cases step with
       | charStep _ _ step => exact .snoc prev (charStep_of_charStep step) cls
 
-theorem reaches_iff_pathIn {nfa : NFA} {i : Fin nfa.nodes.size} {m : List Char} :
-  nfa.reaches i m ↔ nfa.pathIn 0 nfa.start i m := ⟨pathIn_of_reaches, reaches_of_pathIn⟩
-
-theorem matches_of_reaches (eq : compile r = nfa)
-  (h₁ : nfa.reaches i cs) (h₂ : nfa[i] = .done) :
-  r.matches cs := by
-  have hi : i.val = 0 := (done_iff_zero_compile eq i).mp h₂
-  have : nfa.pathIn 0 nfa.start i cs := pathIn_of_reaches h₁
-  simp at this
-  have := pathToNext_of_compile_of_pathIn eq (hi ▸ this)
-  exact (matches_iff_pathToNext eq).mpr this
-
 theorem matches_of_reaches' (eq : compile r = nfa)
   (h₁ : nfa.reaches i cs) (h₂ : nfa[i] = .done) :
   r.matches cs := by
@@ -234,17 +152,6 @@ theorem matches_of_reaches' (eq : compile r = nfa)
     exact ge_pushRegex_start h
   simp [this] at path
   exact (matches_iff_pathIn' eq).mpr (hi ▸ path)
-
-theorem reaches_of_matches (eq : compile r = nfa)
-  (m : r.matches cs) :
-  ∃ i, nfa.reaches i cs ∧ nfa[i] = .done := by
-  have := (matches_iff_pathToNext eq).mp m
-  have := pathIn_of_pathToNext this
-  simp at this
-  let i' : Fin nfa.nodes.size := ⟨0, lt_zero_size_compile eq⟩
-  have := reaches_of_pathIn (i := i') this
-  have hdone := (done_iff_zero_compile eq i').mpr rfl
-  exact ⟨i', this, hdone⟩
 
 theorem reaches_of_matches' (eq : compile r = nfa)
   (m : r.matches cs) :
