RegexCorrectness/NFA/Transition/Path.lean
@@ -1,2 +1,1 @@
 import RegexCorrectness.NFA.Transition.Path.Basic
-import RegexCorrectness.NFA.Transition.Path.Equivalence
